@prefix : <https://www.w3.org/ns/2019/wot/security#> .
@prefix dc: <http://purl.org/dc/elements/1.1/> .
@prefix vs: <http://www.w3.org/2003/06/sw-vocab-status/ns#> .
@prefix owl: <http://www.w3.org/2002/07/owl#> .
@prefix rdf: <http://www.w3.org/1999/02/22-rdf-syntax-ns#> .
@prefix xml: <http://www.w3.org/XML/1998/namespace> .
@prefix xsd: <http://www.w3.org/2001/XMLSchema#> .
@prefix foaf: <http://xmlns.com/foaf/0.1/> .
@prefix prov: <http://www.w3.org/ns/prov#> .
@prefix rdfs: <http://www.w3.org/2000/01/rdf-schema#> .
@prefix vann: <http://purl.org/vocab/vann/> .
@prefix dcterms: <http://purl.org/dc/terms/> .

<https://www.w3.org/2019/wot/security#> rdf:type owl:Ontology ;
                                     
                                     dc:title "Security mechanisms for the Web of Things"@en ;
                                     
                                     vann:preferredNamespacePrefix "wotsec" ;
                                     
                                     vann:preferredNamespaceUri "https://www.w3.org/2019/wot/security#" ;
                                     
                                     owl:versionInfo "0.0.1" ;
                                     
                                     dcterms:license <http://purl.org/NET/rdflicense/cc-by4.0> ;
                                     
                                     dcterms:creator <mailto:michael.mccool@intel.com> ;
                                     
                                     dcterms:contributor <mailto:victor.charpenay@siemens.com> .





#################################################################
#
#    Data properties
#
#################################################################


###  https://www.w3.org/2019/wot/security#alg

<https://www.w3.org/2019/wot/security#alg> rdf:type owl:DatatypeProperty ;
                                        
                                        rdfs:label "alg" ;
                                        
                                        rdfs:comment "Encoding, encryption, or digest algorithm."@en .



###  https://www.w3.org/2019/wot/security#authorization

<https://www.w3.org/2019/wot/security#authorization> rdf:type owl:DatatypeProperty ;
                                                     
                                                     rdfs:label "authorization" ;
                                                     
                                                     rdfs:comment "URI of the authorization server."@en .



###  https://www.w3.org/2019/wot/security#flow

<https://www.w3.org/2019/wot/security#flow> rdf:type owl:DatatypeProperty ;
                                         
                                         rdfs:label "flow" ;
                                         
                                         rdfs:comment "Authorization flow."@en .



###  https://www.w3.org/2019/wot/security#format

<https://www.w3.org/2019/wot/security#format> rdf:type owl:DatatypeProperty ;
                                           
                                           rdfs:label "format" ;
                                           
                                           rdfs:comment "Specifies format of security authentication information."@en .



###  https://www.w3.org/2019/wot/security#identity

<https://www.w3.org/2019/wot/security#identity> rdf:type owl:DatatypeProperty ;
                                             
                                             rdfs:label "identity" ;
                                             
                                             rdfs:comment "Identifier providing information which can be used for selection or confirmation." .



###  https://www.w3.org/2019/wot/security#in

<https://www.w3.org/2019/wot/security#in> rdf:type owl:DatatypeProperty ;
                                       
                                       rdfs:label "in" ;
                                       
                                       rdfs:comment "Specifies the location of security authentication information."@en .



###  https://www.w3.org/2019/wot/security#name

<https://www.w3.org/2019/wot/security#name> rdf:type owl:DatatypeProperty ;
                                         
                                         rdfs:label "name" ;
                                         
                                         rdfs:comment "Name for query, header, or cookie parameters." .



###  https://www.w3.org/2019/wot/security#proxy

<https://www.w3.org/2019/wot/security#proxy> rdf:type owl:DatatypeProperty ;
                                             
                                             rdfs:label "proxy" ;
                                             
                                             rdfs:comment "URI of the proxy server this security configuration provides access to.  If not given, the corresponding security configuration is for the endpoint.  <br/>This feature is at risk."@en .



###  https://www.w3.org/2019/wot/security#qop

<https://www.w3.org/2019/wot/security#qop> rdf:type owl:DatatypeProperty ;
                                        
                                        rdfs:label "qop" ;
                                        
                                        rdfs:comment "Quality of protection.  <br/>This feature is at risk." .



###  https://www.w3.org/2019/wot/security#refresh

<https://www.w3.org/2019/wot/security#refresh> rdf:type owl:DatatypeProperty ;
                                               
                                               rdfs:label "refresh" ;
                                               
                                               rdfs:comment "URI of the refresh server."@en .



###  https://www.w3.org/2019/wot/security#scheme

<https://www.w3.org/2019/wot/security#scheme> rdf:type owl:DatatypeProperty ;
                                           
                                           rdfs:label "scheme" ;
                                           
                                           rdfs:comment "Identification of the security mechanism being configured."@en .



###  https://www.w3.org/2019/wot/security#scopes

<https://www.w3.org/2019/wot/security#scopes> rdf:type owl:DatatypeProperty ;
                                           
                                           rdfs:label "scopes" ;
                                           
                                           rdfs:comment "Set of authorization scope identifiers provided as an array.  These are provided in tokens returned by an authorization server and associated with forms in order to identify what resources a client may access and how.  The values associated with a form should be chosen from those defined in an <code>OAuth2SecurityScheme</code> active on that form.  <br/>This feature is at risk."@en .


###  https://www.w3.org/2019/wot/security#token

<https://www.w3.org/2019/wot/security#token> rdf:type owl:DatatypeProperty ;
                                             
                                             rdfs:label "token" ;
                                             
                                             rdfs:comment "URI of the token server."@en .





#################################################################
#
#    Classes
#
#################################################################


###  https://www.w3.org/2019/wot/security#APIKeySecurityScheme

<https://www.w3.org/2019/wot/security#APIKeySecurityScheme> rdf:type owl:Class ;
                                                         
                                                         rdfs:label "APIKeySecurityScheme" ;
                                                         
                                                         rdfs:subClassOf <https://www.w3.org/2019/wot/security#SecurityScheme> ;
                                                         
                                                         rdfs:comment "API key authentication security configuration identified by the <a>Vocabulary Term</a> <code>apikey</code> (i.e., <code>\"scheme\": \"apikey\"</code>).  This is for the case where the access token is opaque and is not using a standard token format."@en .



###  https://www.w3.org/2019/wot/security#BasicSecurityScheme

<https://www.w3.org/2019/wot/security#BasicSecurityScheme> rdf:type owl:Class ;
                                                        
                                                        rdfs:label "BasicSecurityScheme" ;
                                                        
                                                        rdfs:subClassOf <https://www.w3.org/2019/wot/security#SecurityScheme> ;
                                                        
                                                        rdfs:comment "Basic Authentication [[!RFC7617]] security configuration identified by the <a>Vocabulary Term</a> <code>basic</code> (i.e., <code>\"scheme\": \"basic\"</code>), using an unencrypted username and password.  This scheme should be used with some other security mechanism providing confidentiality, for example, TLS."@en .



###  https://www.w3.org/2019/wot/security#BearerSecurityScheme

<https://www.w3.org/2019/wot/security#BearerSecurityScheme> rdf:type owl:Class ;
                                                         
                                                         rdfs:label "BearerSecurityScheme" ;
                                                         
                                                         rdfs:subClassOf <https://www.w3.org/2019/wot/security#SecurityScheme> ;
                                                         
                                                         rdfs:comment "Bearer Token [[!RFC6750]] security configuration identified by the <a>Vocabulary Term</a> <code>bearer</code> (i.e., <code>\"scheme\": \"bearer\"</code>) for situations where bearer tokens are used independently of OAuth2.  If the <code>oauth2</code> scheme is specified it is not generally necessary to specify this scheme as well as it is implied.  For <code>format</code>, the value <code>jwt</code> indicates conformance with [[!RFC7519]], <code>jws</code> indicates conformance with [[!RFC7797]], <code>cwt</code> indicates conformance with [[!RFC8392]], and <code>jwe</code> indicates conformance with [[!RFC7516]], with values for <code>alg</code> interpreted consistently with those standards. <span class=\"rfc2119-assertion\" id=\"td-security-bearer-format-extensions\">Other formats and algorithms for bearer tokens MAY be specified in vocabulary extensions.</span>" .

###  https://www.w3.org/2019/wot/security#CertSecurityScheme

<https://www.w3.org/2019/wot/security#CertSecurityScheme> rdf:type owl:Class ;
                                                      
                                                      rdfs:label "CertSecurityScheme" ;
                                                      
                                                      rdfs:subClassOf <https://www.w3.org/2019/wot/security#SecurityScheme> ;
                                                      
                                                      rdfs:comment "Certificate-based asymmetric key security configuration conformant with [[!X509V3]] identified by the <a>Vocabulary Term</a> <code>cert</code> (i.e., <code>\"scheme\": \"cert\"</code>)." .



###  https://www.w3.org/2019/wot/security#DigestSecurityScheme

<https://www.w3.org/2019/wot/security#DigestSecurityScheme> rdf:type owl:Class ;
                                                         
                                                         rdfs:label "DigestSecurityScheme" ;
                                                         
                                                         rdfs:subClassOf <https://www.w3.org/2019/wot/security#SecurityScheme> ;
                                                         
                                                         rdfs:comment "Digest Access Authentication [[!RFC7616]] security configuration identified by the <a>Vocabulary Term</a> <code>digest</code> (i.e., <code>\"scheme\": \"digest\"</code>). This scheme is similar to basic authentication but with added features to avoid man-in-the-middle attacks." .



###  https://www.w3.org/2019/wot/security#NoSecurityScheme

<https://www.w3.org/2019/wot/security#NoSecurityScheme> rdf:type owl:Class ;
                                                       
                                                       rdfs:label "NoSecurityScheme" ;
                                                       
                                                       rdfs:subClassOf <https://www.w3.org/2019/wot/security#SecurityScheme> ;
                                                       
                                                       rdfs:comment "A security configuration corresponding to identified by the <a>Vocabulary Term</a> <code>nosec</code> (i.e., <code>\"scheme\": \"nosec\"</code>), indicating there is no authentication or other mechanism required to access the resource."@en .



###  https://www.w3.org/2019/wot/security#OAuth2SecurityScheme

<https://www.w3.org/2019/wot/security#OAuth2SecurityScheme> rdf:type owl:Class ;
                                                         
                                                         rdfs:label "OAuth2SecurityScheme" ;
                                                         
                                                         rdfs:subClassOf <https://www.w3.org/2019/wot/security#SecurityScheme> ;
                                                         
                                                         rdfs:comment "OAuth2 authentication security configuration for systems conformant with [[!RFC6749]] and [[!RFC8252]], identified by the <a>Vocabulary Term</a> <code>oauth2</code> (i.e., <code>\"scheme\": \"oauth2\"</code>).  <span class=\"rfc2119-assertion\" id=\"td-security-oauth2-implicit-flow\">For the <code>implicit</code> flow <code>authorization</code> MUST be included.</span>  <span class=\"rfc2119-assertion\" id=\"td-security-oauth2-password-client-flow\">For the <code>password</code> and <code>client</code> flows <code>token</code> MUST be included.</span>  <span class=\"rfc2119-assertion\" id=\"td-security-oauth2-code-flow\">For the <code>code</code> flow both <code>authorization</code> and <code>token</code> MUST be included.</span>  If no <code>scopes</code> are defined in the <code>SecurityScheme</code> then they are considered to be empty."@en .



###  https://www.w3.org/2019/wot/security#PSKSecurityScheme

<https://www.w3.org/2019/wot/security#PSKSecurityScheme> rdf:type owl:Class ;
                                                      
                                                      rdfs:label "PSKSecurityScheme" ;
                                                      
                                                      rdfs:subClassOf <https://www.w3.org/2019/wot/security#SecurityScheme> ;
                                                      
                                                      rdfs:comment "Pre-shared key authentication security configuration identified by the <a>Vocabulary Term</a> <code>psk</code> (i.e., <code>\"scheme\": \"psk\"</code>)." .



###  https://www.w3.org/2019/wot/security#PoPSecurityScheme

<https://www.w3.org/2019/wot/security#PoPSecurityScheme> rdf:type owl:Class ;
                                                      
                                                      rdfs:label "PoPSecurityScheme" ;
                                                      
                                                      rdfs:subClassOf <https://www.w3.org/2019/wot/security#SecurityScheme> ;
                                                      
                                                      rdfs:comment "Proof-of-possession (PoP) token authentication security configuration identified by the <a>Vocabulary Term</a> <code>pop</code> (i.e., <code>\"scheme\": \"pop\"</code>). Here <code>jwt</code> indicates conformance with [[!RFC7519]], <code>jws</code> indicates conformance with [[!RFC7797]], <code>cwt</code> indicates conformance with [[!RFC8392]], and <code>jwe</code> indicates conformance with [[!RFC7516]], with values for <code>alg</code> interpreted consistently with those standards. <span class=\"rfc2119-assertion\" id=\"td-security-pop-format-extensions\">Other formats and algorithms for PoP tokens MAY be specified in vocabulary extensions.</span>" .

###  https://www.w3.org/2019/wot/security#PublicSecurityScheme

<https://www.w3.org/2019/wot/security#PublicSecurityScheme> rdf:type owl:Class ;
                                                      
                                                      rdfs:label "PublicSecurityScheme" ;
                                                      
                                                      rdfs:subClassOf <https://www.w3.org/2019/wot/security#SecurityScheme> ;
                                                      
                                                      rdfs:comment "Raw public key asymmetric key security configuration identified by the <a>Vocabulary Term</a> <code>public</code> (i.e., <code>\"scheme\": \"public\"</code>)." .



###  https://www.w3.org/2019/wot/security#SecurityScheme

<https://www.w3.org/2019/wot/security#SecurityScheme> rdf:type owl:Class ;

rdfs:comment "Metadata describing the configuration of a security mechanism.  <span class=\"rfc2119-assertion\" id=\"td-security-scheme-name\">The value assigned to the name <code>scheme</code> MUST be defined within a <a>Vocabulary</a> included in the <a>Thing Description</a>, either in the standard <a>Vocabulary</a> defined in <a href=\"#sec-vocabulary-definition\"></a> or in a <a>TD Context Extension</a>." .
###  Generated by the OWL API (version 3.4.2) http://owlapi.sourceforge.net

